Memory.v
@@ -1,49 +1,38 @@
 Require Import Datatypes.
 Require Import ZArith.
-Require Import List.
-Require Import EquivDec.
 Require Import String.
 Require Import Show.
 
 Require Import Utils.
 
-Fixpoint replicate {A:Type} (n:nat) (a:A) : list A :=
-  match n with
-    | O => nil
-    | S n' => a :: replicate n' a
-  end.
+Require Import ssreflect ssrbool ssrfun ssrnat eqtype seq.
 
-Definition zreplicate {A:Type} (n:Z) (a:A) : option (list A) :=
+Definition zreplicate {A:Type} (n:Z) (a:A) : option (seq A) :=
   if Z_lt_dec n 0 then None
-  else Some (replicate (Z.to_nat n) a).
-
-Lemma nth_error_replicate: forall A n (a:A) n',
-  nth_error (replicate n a) n' = if lt_dec n' n then Some a else None.
-Proof.
-  induction n; destruct n'; simpl; try reflexivity.
-  rewrite IHn.
-  do 2 destruct lt_dec; try congruence; try omega.
-Qed.
+  else Some (nseq (Z.to_nat n) a).
 
 Lemma nth_error_Z_zreplicate: forall A z (a:A) z' l,
   zreplicate z a = Some l ->
   nth_error_Z l z' = if Z_le_dec 0 z' then
-                        if Z_lt_dec z' z then Some a else None else None.
+                        if Z_lt_dec z' z then Some a else None
+                     else None.
 Proof.
   unfold zreplicate, nth_error_Z; intros.
   destruct (Z_lt_dec z 0); try congruence.
   inv H.
   destruct (z' <? 0)%Z eqn:Ez.
-  - rewrite Z.ltb_lt in Ez.
+  - rewrite -> Z.ltb_lt in Ez.
     destruct Z_lt_dec; try omega.
     destruct Z_le_dec; auto; omega.
   - assert (~ (z' < 0 )%Z).
     rewrite <- Z.ltb_lt; try congruence.
-    destruct Z_le_dec; try omega.
-    rewrite nth_error_replicate.
-    assert ( (z'<z)%Z <-> (Z.to_nat z') < (Z.to_nat z)).
+    destruct Z_le_dec; try omega; simpl in *; inv H.
+    rewrite (_ : is_left (Z_lt_dec z' z) = (Z.to_nat z' < Z.to_nat z)).
+      elim: (Z.to_nat z') (Z.to_nat z) {n Ez H0 l0}=> [|n IH] [|n'] //=.
+      by rewrite IH ltnS.
+    assert ( (z'<z)%Z <-> (Z.to_nat z' < Z.to_nat z)%coq_nat).
       apply Z2Nat.inj_lt; try omega.
-    destruct lt_dec; destruct Z_lt_dec; auto; try omega.
+    by apply/sumboolP/ltP; intuition.
 Qed.
 
 Inductive alloc_mode := Global | Local.
@@ -52,16 +41,22 @@ Inductive alloc_mode := Global | Local.
 (* Cannot make this a parameter because we don't want it opaque.
    Keep it outside for now, until I figure out what's better *)
 (* Any better solutions than the implicit arguments welcome *)
-Inductive frame {A S} := Fr (stamp : S) (label : S) : list A -> @frame A S.
-
+Inductive frame {A S} := Fr (stamp : S) (label : S) : seq A -> @frame A S.
 
 Module Type MEM.
   (* Type of memory is parameterized by the type of stamps and the type of block *)
   Parameter t : Type -> Type -> Type.
 
   Parameter block : Type -> Type.
-  Declare Instance EqDec_block : forall {S} {_:EqDec S eq}, EqDec (block S) eq.
   Parameter stamp : forall {S}, block S -> S.
+
+  Parameter block_eq : forall (S : eqType), block S -> block S -> bool.
+
+  Parameter block_eqP : forall S, Equality.axiom (@block_eq S).
+
+  Definition block_eqMixin (S : eqType) := EqMixin (block_eqP S).
+  Canonical block_eqType (S : eqType) :=
+    EqType (block S) (block_eqMixin S).
 
   (* For generation *)
   Parameter put_stamp : forall {S}, S -> block S -> block S.
@@ -74,31 +69,31 @@ Module Type MEM.
   (* DD -> DP : is a block some kind of "stamped pointer"? *)
   Parameter get_frame : forall {A S}, t A S -> block S -> option (@frame A S).
   Parameter upd_frame :
-    forall {A S:Type} {EqS:EqDec S eq}, t A S -> block S -> @frame A S ->
-                                        option (t A S).
-  Parameter upd_get_frame : forall A S (EqS:EqDec S eq) (m:t A S) (b:block S) fr fr',
+    forall {A} {S:eqType}, t A S -> block S -> @frame A S -> option (t A S).
+
+  Parameter upd_get_frame : forall A (S : eqType) (m:t A S) (b:block S) fr fr',
     get_frame m b = Some fr ->
     exists m',
       upd_frame m b fr' = Some m'.
-  Parameter get_upd_frame : forall A S (EqS:EqDec S eq) (m m':t A S) (b:block S) fr,
+  Parameter get_upd_frame : forall A (S : eqType) (m m':t A S) (b:block S) fr,
     upd_frame m b fr = Some m' ->
     forall b',
       get_frame m' b' = if b == b' then Some fr else get_frame m b'.
-  Parameter upd_frame_defined : forall A S (EqS:EqDec S eq) (m m':t A S) (b:block S) fr,
+  Parameter upd_frame_defined : forall A (S : eqType) (m m':t A S) (b:block S) fr,
     upd_frame m b fr = Some m' ->
     exists fr', get_frame m b = Some fr'.
 
-  Parameter memory_extensionality : 
-    forall {A S} {_:EqDec S eq} (m1 m2 : t A S),
+  Parameter memory_extensionality :
+    forall {A} {S : eqType} (m1 m2 : t A S),
     (forall (b : block S), get_frame m1 b = get_frame m2 b) -> m1 = m2.
 
-  Parameter get_blocks : forall {A S} , list S -> t A S -> list (block S).
+  Parameter get_blocks : forall {A S} , seq S -> t A S -> seq (block S).
 
   Parameter get_blocks_spec:
-    forall {A S} (labs : list S) (mem: t A S) (b: block S),
-      In (stamp b) labs /\
+    forall {A} {S : eqType} (labs : seq S) (mem: t A S) (b: block S),
+      stamp b \in labs /\
       (exists fr, get_frame mem b = Some fr) <->
-      In b (get_blocks labs mem).
+      b \in get_blocks labs mem.
 
   Parameter empty : forall A S, t A S.
   Parameter get_empty : forall A S (b:block S), get_frame (empty A S) b = None.
@@ -120,32 +115,32 @@ Module Type MEM.
   (*                            get_frame (init A S mode b f) b' = None. *)
 
   Parameter alloc :
-    forall {A S} {EqS:EqDec S eq}, alloc_mode -> t A S -> S -> @frame A S -> (block S * t A S).
-  Parameter alloc_stamp : forall A S (EqS:EqDec S eq) am (m m':t A S) s fr b,
+    forall {A} {S : eqType}, alloc_mode -> t A S -> S -> @frame A S -> (block S * t A S).
+  Parameter alloc_stamp : forall A (S : eqType) am (m m':t A S) s fr b,
     alloc am m s fr = (b,m') -> stamp b = s.
-  Parameter alloc_get_fresh : forall A S (EqS:EqDec S eq) am (m m':t A S) s fr b,
+  Parameter alloc_get_fresh : forall A (S : eqType) am (m m':t A S) s fr b,
     alloc am m s fr = (b,m') -> get_frame m b = None.
-  Parameter alloc_get_frame : forall A S (eqS:EqDec S eq) am (m m':t A S) s fr b,
+  Parameter alloc_get_frame : forall A (S : eqType) am (m m':t A S) s fr b,
     alloc am m s fr = (b,m') ->
     forall b', get_frame m' b' = if b == b' then Some fr else get_frame m b'.
-  Parameter alloc_upd : forall A S (eqS:EqDec S eq) am (m:t A S) b fr1 s fr2 m',
+  Parameter alloc_upd : forall A (S : eqType) am (m:t A S) b fr1 s fr2 m',
     upd_frame m b fr1 = Some m' ->
     fst (alloc am m' s fr2) = fst (alloc am m s fr2).
   Parameter alloc_local_comm :
-    forall A S (EqS:EqDec S eq)  (m m1 m2 m1' m2':t A S) s s' fr fr' b1 b2 b1',
+    forall A (S : eqType) (m m1 m2 m1' m2':t A S) s s' fr fr' b1 b2 b1',
     s <> s' ->
     alloc Local m s fr = (b1,m1) ->
     alloc Local m1 s' fr' = (b2,m2) ->
     alloc Local m s' fr' = (b1',m1') ->
     b1' = b2.
   Parameter alloc2_local :
-    forall A S (EqS:EqDec S eq)  (m1 m2 m1' m2':t A S) s fr1 fr2 fr' b,
+    forall A (S : eqType) (m1 m2 m1' m2':t A S) s fr1 fr2 fr' b,
     alloc Local m1 s fr1 = (b,m1') ->
     alloc Local m2 s fr2 = (b,m2') ->
     fst (alloc Local m1' s fr') = fst (alloc Local m2' s fr').
 
   Parameter alloc_next_block_no_fr :
-    forall A S (EqS:EqDec S eq) (m:t A S) s fr1 fr2,
+    forall A (S : eqType) (m:t A S) s fr1 fr2,
     fst (alloc Local m s fr1) = fst (alloc Local m s fr2).
 
   Parameter map : forall {A B S}, (@frame A S -> @frame B S) -> t A S -> t B S.
@@ -159,17 +154,16 @@ End MEM.
 Module Mem: MEM.
   Definition block S := (Z * S)%type.
 
-  Instance EqDec_block : forall {S} {EqS:EqDec S eq}, EqDec (block S) eq.
-  Proof.
-    intros S E (x,s) (x',s').
-    destruct (Z.eq_dec x x').
-    destruct (s == s').
-    left; congruence.
-    right; congruence.
-    right; congruence.
-  Qed.
+  Definition block_eq (S : eqType) (b1 b2 : block S) := b1 == b2.
 
-  Definition stamp S : block S -> S := snd.
+  Lemma block_eqP (S : eqType) : Equality.axiom (@block_eq S).
+  Proof. move=> ??; exact/eqP. Qed.
+
+  Definition block_eqMixin (S : eqType) := EqMixin (block_eqP S).
+  Canonical block_eqType (S : eqType) :=
+    EqType (block S) (block_eqMixin S).
+
+  Definition stamp S : block S -> S := @snd _ _.
   Definition put_stamp S (s : S) (b : block S) : block S :=
     let (z,_) := b in (z,s).
 
@@ -190,27 +184,20 @@ Module Mem: MEM.
 
   Definition get_frame {A S} (m:t A S) := content m.
 
-  Definition memory_extensionality {A S} {_ : EqDec S eq} (m1 m2 : t A S) 
+  Definition memory_extensionality {A} {S : eqType} (m1 m2 : t A S)
              (H : forall b, get_frame m1 b = get_frame m2 b) : m1 = m2.
     admit.
   Qed.
 
-  Definition Z_seq z1 z2 := map Z.of_nat (seq (Z.to_nat z1) (Z.to_nat z2)).
-
-  Fixpoint list_of_option {A : Type} (l : list (option A)) : list A :=
-    match l with
-      | nil => nil
-      | Some h :: t => h :: list_of_option t
-      | None :: t => list_of_option t
-    end.
+  Definition Z_seq z1 z2 := map Z.of_nat (iota (Z.to_nat z1) (Z.to_nat z2)).
 
   Definition get_blocks_at_level {A S} (m : t A S) (s : S):=
     let max := next m s in
     let indices := Z_seq 1%Z (max - 1) in
     map (fun ind => (ind,s)) indices.
 
-  Definition get_blocks {A S} (ss : list S) (m : t A S) : list (block S) :=
-    flat_map (get_blocks_at_level m) ss.
+  Definition get_blocks {A S} (ss : list S) (m : t A S) : seq (block S) :=
+    flatten (map (get_blocks_at_level m) ss).
 
   Instance show_block {S} {_: Show S}: Show (block S) :=
   {|
@@ -221,7 +208,7 @@ Module Mem: MEM.
 
   Program Definition map {A B S} (f:@frame A S -> @frame B S) (m:t A S) : t B S:=
     MEM
-      (fun b => option_map f (get_frame m b))
+      (fun b => omap f (get_frame m b))
       (next m)
       _ _.
   Next Obligation.
@@ -237,7 +224,7 @@ Module Mem: MEM.
   Qed.
 
   Lemma map_spec : forall A B S (f:@frame A S -> @frame B S) (m:t A S),
-    forall b, get_frame (map f m) b = option_map f (get_frame m b).
+    forall b, get_frame (map f m) b = omap f (get_frame m b).
   Proof.
     auto.
   Qed.
@@ -291,7 +278,7 @@ Module Mem: MEM.
   (*   end. *)
   (* Qed. *)
 
-  Program Definition upd_frame_rich {A S} {EqS:EqDec S eq} (m:t A S) (b0:block S) (fr:@frame A S)
+  Program Definition upd_frame_rich {A} {S : eqType} (m:t A S) (b0:block S) (fr:@frame A S)
   : option { m' : (t A S) |
              (forall b',
                 get_frame m' b' = if b0 == b' then Some fr else get_frame m b')
@@ -305,44 +292,42 @@ Module Mem: MEM.
     end.
   Next Obligation.
     split.
-    - destruct (equiv_dec b0).
+    - have [e|ne] := altP (b0 =P _).
       + destruct b0; inv e. eexists. reflexivity.
       + apply content_next; auto.
-    - intros [fr' Hif].
-      destruct b0.
-      destruct (equiv_dec (z,s0) (i, s)). inv e.
-      destruct (content_next m s i) as [_ H]. apply H.
-      eexists. symmetry. exact Heq_anonymous.
-      destruct (content_next m s i) as [_ H]. apply H.
-      eexists. eassumption.
+    - have [e|ne] := altP (b0 =P _).
+      + case=> [? [?]]; inv e.
+        destruct (content_next m s i) as [_ H]. apply H.
+        eexists. symmetry. exact Heq_anonymous.
+      + destruct (content_next m s i) as [_ H]. apply H.
   Qed.
   Next Obligation.
     destruct m. auto.
   Qed.
 
-  Definition upd_frame {A S} {EqS:EqDec S eq} (m:t A S) (b0:block S) (fr:@frame A S)
+  Definition upd_frame {A} {S : eqType} (m:t A S) (b0:block S) (fr:@frame A S)
   : option (t A S) :=
     match upd_frame_rich m b0 fr with
       | None => None
       | Some (exist m' _) => Some m'
     end.
 
-  Program Lemma upd_get_frame : forall A S (EqS:EqDec S eq) (m:t A S) (b:block S) fr fr',
+  Program Lemma upd_get_frame : forall A (S : eqType) (m:t A S) (b:block S) fr fr',
     get_frame m b = Some fr ->
     exists m',
       upd_frame m b fr' = Some m'.
   Proof.
     unfold upd_frame, upd_frame_rich, get_frame.
     intros.
-    generalize (@eq_refl (option (@frame A S)) (m b)).
-    generalize (upd_frame_rich_obligation_3 A S EqS m b fr').
-    generalize (upd_frame_rich_obligation_2 A S EqS m b fr').
-    generalize (upd_frame_rich_obligation_1 A S EqS m b fr').
+    generalize (@erefl (option (@frame A S)) (m b)).
+    generalize (upd_frame_rich_obligation_3 A S m b fr').
+    generalize (upd_frame_rich_obligation_2 A S m b fr').
+    generalize (upd_frame_rich_obligation_1 A S m b fr').
     simpl.
     rewrite H. intros. eauto.
   Qed.
 
-  Lemma get_upd_frame : forall A S (eqS:EqDec S eq) (m m':t A S) (b:block S) fr,
+  Lemma get_upd_frame : forall A (S : eqType) (m m':t A S) (b:block S) fr,
     upd_frame m b fr = Some m' ->
     forall b',
       get_frame m' b' = if b == b' then Some fr else get_frame m b'.
@@ -352,16 +337,16 @@ Module Mem: MEM.
     destruct s; inv H; intuition.
   Qed.
 
-  Lemma upd_frame_defined : forall A S (EqS:EqDec S eq) (m m':t A S) (b:block S) fr,
+  Lemma upd_frame_defined : forall A (S : eqType) (m m':t A S) (b:block S) fr,
     upd_frame m b fr = Some m' ->
     exists fr', get_frame m b = Some fr'.
   Proof.
     unfold upd_frame, upd_frame_rich, get_frame.
     intros until 0.
-    generalize (@eq_refl (option (@frame A S)) (@content A S m b)).
-    generalize (upd_frame_rich_obligation_3 A S EqS m b fr).
-    generalize (upd_frame_rich_obligation_2 A S EqS m b fr).
-    generalize (upd_frame_rich_obligation_1 A S EqS m b fr).
+    generalize (@erefl (option (@frame A S)) (@content A S m b)).
+    generalize (upd_frame_rich_obligation_3 A S m b fr).
+    generalize (upd_frame_rich_obligation_2 A S m b fr).
+    generalize (upd_frame_rich_obligation_1 A S m b fr).
     simpl.
     intros.
     destruct (m b); eauto; congruence.
@@ -370,7 +355,7 @@ Module Mem: MEM.
   Opaque Z.add.
 
   Program Definition alloc
-             {A S} {EqS:EqDec S eq} (am:alloc_mode) (m:t A S) (s:S) (fr:@frame A S)
+             {A} {S : eqType} (am:alloc_mode) (m:t A S) (s:S) (fr:@frame A S)
             : (block S * t A S) :=
     ((next m s,s),
      MEM
@@ -378,22 +363,20 @@ Module Mem: MEM.
        (fun s' => if s == s' then (1 + next m s)%Z else next m s')
        _ _).
   Next Obligation.
-    destruct (equiv_dec (next m s, s)).
-    - inv e. split.
-      + destruct (equiv_dec s0); try congruence.
-        intros Hrng. eexists. reflexivity.
+    have [e|ne] := (next m s, s) =P _.
+    - inv e; rewrite eqxx; split.
+      + intros Hrng. eexists. reflexivity.
       + intros [fr' Heq]. inv Heq. split.
-        apply next_pos.
-        destruct (equiv_dec s0 s0). omega. congruence.
-    - destruct (equiv_dec s s0).
+        apply next_pos. omega.
+    - have [e|ne'] := s =P s0.
       + inv e. split.
         * intros [Hrng1 Hrng2]. destruct (content_next m s0 i) as [H _].
-          apply H. compute in c. split. assumption.
+          apply H. split; first assumption.
           apply Zlt_is_le_bool in Hrng2.
-          rewrite Z.add_comm, <- Z.add_sub_assoc, Z.add_0_r in Hrng2.
+          rewrite -> Z.add_comm, <- Z.add_sub_assoc, Z.add_0_r in Hrng2.
           apply Zle_bool_imp_le in Hrng2. apply Zle_lt_or_eq in Hrng2.
           destruct Hrng2 as [Hrng2 | Hrng2]. assumption.
-          subst. exfalso. apply c. reflexivity.
+          subst. exfalso. apply ne. reflexivity.
         * intros [fr' Heq]. destruct (content_next m s0 i) as [_ H].
           unfold get_frame in Heq.
           assert (ex: (exists fr0 : frame, m (i, s0) = Some fr0))
@@ -402,20 +385,19 @@ Module Mem: MEM.
       + split; intro Hrng; destruct (content_next m s0 i) as [H1 H2]; auto.
   Qed.
   Next Obligation.
-    destruct (equiv_dec s s0);
-    destruct m; simpl.
+    have [e|ne] := s =P s0; destruct m; simpl.
     - specialize (next_pos0 s); try omega.
     - specialize (next_pos0 s0); assumption.
   Qed.
 
-  Lemma alloc_stamp : forall A S (EqS:EqDec S eq) am (m m':t A S) s fr b,
+  Lemma alloc_stamp : forall A (S : eqType) am (m m':t A S) s fr b,
     alloc am m s fr = (b,m') -> stamp _ b = s.
   Proof.
     unfold alloc; intros.
     inv H; auto.
   Qed.
 
-  Lemma alloc_get_fresh : forall A S (EqS:EqDec S eq) am (m m':t A S) s fr b,
+  Lemma alloc_get_fresh : forall A (S : eqType) am (m m':t A S) s fr b,
     alloc am m s fr = (b,m') -> get_frame m b = None.
   Proof.
     unfold alloc; intros.
@@ -429,7 +411,7 @@ Module Mem: MEM.
     - reflexivity.
   Qed.
 
-  Lemma alloc_get_frame : forall A S (eqS:EqDec S eq) am (m m':t A S) s fr b,
+  Lemma alloc_get_frame : forall A (S : eqType) am (m m':t A S) s fr b,
     alloc am m s fr = (b,m') ->
     forall b', get_frame m' b' = if b == b' then Some fr else get_frame m b'.
   Proof.
@@ -437,11 +419,11 @@ Module Mem: MEM.
     inv H; auto.
   Qed.
 
-  Lemma alloc_upd : forall A S (eqS:EqDec S eq) am (m:t A S) b fr1 s fr2 m',
+  Lemma alloc_upd : forall A (S : eqType) am (m:t A S) b fr1 s fr2 m',
     upd_frame m b fr1 = Some m' ->
     fst (alloc am m' s fr2) = fst (alloc am m s fr2).
   Proof.
-    intros A S eqS am m b fr1 s fr2 m' H.
+    intros A S am m b fr1 s fr2 m' H.
     unfold alloc, upd_frame in *; simpl.
     destruct (upd_frame_rich m b fr1); try congruence.
     destruct s0; inv H.
@@ -450,34 +432,34 @@ Module Mem: MEM.
   Qed.
 
   Lemma alloc_local_comm :
-    forall A S (EqS:EqDec S eq) (m m1 m2 m1' m2':t A S) s s' fr fr' b1 b2 b1',
+    forall A (S : eqType) (m m1 m2 m1' m2':t A S) s s' fr fr' b1 b2 b1',
     s <> s' ->
     alloc Local m s fr = (b1,m1) ->
     alloc Local m1 s' fr' = (b2,m2) ->
     alloc Local m s' fr' = (b1',m1') ->
     b1' = b2.
   Proof.
-    intros A S EqS m m1 m2 m1' m2' s s' fr fr' b1 b2 b1' H H0 H1 H2.
+    intros A S m m1 m2 m1' m2' s s' fr fr' b1 b2 b1' H H0 H1 H2.
     inv H0; inv H1; inv H2.
-    destruct (equiv_dec s s'); try congruence.
+    destruct (s =P s'); try congruence.
   Qed.
 
   Lemma alloc2_local :
-    forall A S (EqS:EqDec S eq)  (m1 m2 m1' m2':t A S) s fr1 fr2 fr' b,
+    forall A (S : eqType) (m1 m2 m1' m2':t A S) s fr1 fr2 fr' b,
     alloc Local m1 s fr1 = (b,m1') ->
     alloc Local m2 s fr2 = (b,m2') ->
     fst (alloc Local m1' s fr') = fst (alloc Local m2' s fr').
   Proof.
-    intros A S EqS m1 m2 m1' m2' s fr1 fr2 fr' b H H0.
+    intros A S m1 m2 m1' m2' s fr1 fr2 fr' b H H0.
     inv H; inv H0; simpl.
     rewrite H1; auto.
   Qed.
 
   Lemma alloc_next_block_no_fr :
-    forall A S (EqS:EqDec S eq) (m:t A S) s fr1 fr2,
+    forall A (S : eqType) (m:t A S) s fr1 fr2,
     fst (alloc Local m s fr1) = fst (alloc Local m s fr2).
   Proof.
-    intros A S EqS m s fr1 fr2.
+    intros A S m s fr1 fr2.
     unfold alloc; simpl; auto.
   Qed.
 
@@ -486,12 +468,11 @@ Module Mem: MEM.
       (0 <= start)%Z ->
       (0 <= len)%Z ->
       ((start <= z < len + start)%Z <->
-       In z (Z_seq start len)).
+       z \in (Z_seq start len)).
   Proof.
     intros z s l. intros Hle1 Hle2. split.
     - intros [H1 H2]. unfold Z_seq.
-      apply in_map_iff. exists (Z.to_nat z).
-      split. apply Z2Nat.id. omega.
+      apply/mapP. exists (Z.to_nat z); last by rewrite Z2Nat.id; omega.
       apply Z2Nat.inj_lt in H2; try omega.
       rewrite Z2Nat.inj_add in H2; try omega.
       apply Z2Nat.inj_le in H1; try omega.
@@ -504,16 +485,16 @@ Module Mem: MEM.
       induction len as [| l IHl]; intros s start Hle1 Hle3.
       + omega.
       + simpl in *. apply le_lt_or_eq in Hle1. destruct Hle1 as [H1 | H2].
-        right. apply IHl; try omega.
-        left. assumption.
+        rewrite inE; apply/orP; right. apply IHl; try omega.
+        rewrite inE; apply/orP; left; apply/eqP; congruence.
     - intros HIn. unfold Z_seq in HIn.
-      apply in_map_iff in HIn. destruct HIn as [z' [Heq HIn]]. subst.
+      move/mapP in HIn. destruct HIn as [z' HIn Heq]. subst.
       assert (H: Z.to_nat s <= z' < (Z.to_nat l) + (Z.to_nat s) ->
                  (s <= (Z.of_nat z') < l + s)%Z).
-      { intros [H1 H2]. split.
-        apply Z2Nat.inj_le; try omega. rewrite Nat2Z.id. assumption.
-        apply Z2Nat.inj_lt; try omega. rewrite Nat2Z.id, Z2Nat.inj_add;
-         try omega; assumption. }
+      { move=> /andP [H1 H2]. split.
+        apply Z2Nat.inj_le; try omega. rewrite Nat2Z.id. apply/leP. assumption.
+        apply Z2Nat.inj_lt; try omega. rewrite Nat2Z.id Z2Nat.inj_add;
+         try omega. apply/ltP. assumption. }
       apply H.
       apply Z2Nat.inj_le in Hle1; try omega.
       apply Z2Nat.inj_le in Hle2; try omega.
@@ -522,39 +503,90 @@ Module Mem: MEM.
       clear H Heqlen l Heqstart s.
       generalize dependent start. generalize dependent z'.
       induction len as [| len IHlen].
-      + contradiction.
-      + intros z' start Hle HIn. simpl in *.
-        destruct HIn. subst. split; omega.
-        rewrite plus_n_Sm.
+      + by [].
+      + intros z' start Hle; rewrite /= inE => /orP HIn. simpl in *.
+        case: HIn => [/eqP ?|HIn]; subst.
+          rewrite addnE /addn_rec; apply/andP; split; [apply/leP|apply/ltP]; omega.
+        * rewrite addSn -addnS.
         assert (H': S start <= z' < len + S start ->
                     start <= z' < len + S start).
-        { intros [H1 H2]. split; try omega. }
+        { rewrite addnE /addn_rec.
+          move=> /andP [/leP H1 /ltP H2].
+          apply/andP; split; [apply/leP| apply/ltP]; try omega. }
         apply H'. apply IHlen; try omega. assumption.
   Qed.
 
   Lemma get_blocks_spec :
-    forall A S (labs : list S) (mem: t A S) b,
-      In (stamp _ b) labs /\
+    forall A (S : eqType) (labs : seq S) (mem: t A S) b,
+      stamp _ b \in labs /\
       (exists fr, get_frame mem b = Some fr) <->
-      In b (get_blocks labs mem).
+      b \in get_blocks labs mem.
   Proof.
     intros A S labs mem b.
     split.
     - intros [HIn [fr Hget]].
-      unfold get_blocks. apply in_flat_map. eexists; split; [eassumption |].
-      unfold get_blocks_at_level. apply in_map_iff. exists (fst b);
-      destruct b; simpl; split.
-      + reflexivity.
-      + apply in_seq_Z; try omega.
-        * apply Zle_minus_le_0. apply next_pos.
-        * rewrite <- Z.sub_sub_distr, Z.sub_0_r. simpl.
-          apply content_next. eexists. eassumption.
+      unfold get_blocks; apply/flatten_mapP.
+      eexists; [eassumption|].
+      unfold get_blocks_at_level. apply/mapP. exists b.1;
+      destruct b=> //.
+      apply in_seq_Z; try omega.
+      * apply Zle_minus_le_0. apply next_pos.
+      * rewrite <- Z.sub_sub_distr, Z.sub_0_r. simpl.
+        apply content_next. eexists. eassumption.
     - intros HIn. unfold get_blocks, get_blocks_at_level in *.
-      apply in_flat_map in HIn. destruct HIn as [l [HInl HIn]].
-      apply in_map_iff in HIn. destruct HIn as [z [Heq HIn]]. subst.
+      move/flatten_mapP in HIn. destruct HIn as [l HInl HIn].
+      move/mapP in HIn. destruct HIn as [z HIn Heq]. subst.
       split. assumption.
       unfold get_frame. apply content_next. apply in_seq_Z in HIn; try omega.
       apply Zle_minus_le_0. apply next_pos.
   Qed.
 
 End Mem.
+
+Canonical Mem.block_eqType.
+
+Lemma alloc_get_frame_old :
+  forall T (S : eqType) mode mem (stamp : S) (f f' : @frame T S) b b' mem'
+         (ALLOC : Mem.alloc mode mem stamp f' = (b', mem'))
+         (FRAME : Mem.get_frame mem b = Some f),
+    Mem.get_frame mem' b = Some f.
+Proof.
+  intros.
+  erewrite Mem.alloc_get_frame; eauto.
+  have [e|//] := altP (b' =P b).
+  exploit Mem.alloc_get_fresh; eauto.
+  congruence.
+Qed.
+
+Lemma alloc_get_frame_new :
+  forall T (S : eqType) mode mem (stamp : S) (frame : @frame T S) b mem'
+         (ALLOC : Mem.alloc mode mem stamp frame = (b, mem')),
+    Mem.get_frame mem' b = Some frame.
+Proof.
+  intros.
+  erewrite Mem.alloc_get_frame; eauto.
+  by rewrite eqxx; simpl in *; auto.
+Qed.
+
+Lemma get_frame_upd_frame_eq :
+  forall T (S : eqType)
+         (m : Mem.t T S) b f m'
+         (UPD : Mem.upd_frame m b f = Some m'),
+    Mem.get_frame m' b = Some f.
+Proof.
+  intros.
+  erewrite Mem.get_upd_frame; eauto.
+  by rewrite eqxx.
+Qed.
+
+Lemma get_frame_upd_frame_neq :
+  forall T (S : eqType)
+         (m : Mem.t T S) b b' f m'
+         (UPD : Mem.upd_frame m b f = Some m')
+         (NEQ : b' <> b),
+    Mem.get_frame m' b' = Mem.get_frame m b'.
+Proof.
+  intros.
+  erewrite Mem.get_upd_frame; eauto.
+  have [?|?] := (b =P b'); simpl in *; congruence.
+Qed.
