Lab2.v
@@ -1,5 +1,5 @@
 Require Import Labels.
-Require Import List. Import ListNotations.
+Require Import ssreflect ssrbool ssrfun eqtype seq.
 
 (** The two point finite lattice *)
 Inductive Lab2 : Set :=
@@ -20,15 +20,20 @@ Instance JoinSemiLattice_Lab2 : JoinSemiLattice Lab2 :=
       | _, H => true
       | _, _ => false
     end
+; meet l1 l2 :=
+    match l1, l2 with
+    | L, _ => L
+    | _, L => L
+    | H, H => H
+    end
 }.
 Proof.
 auto.
 intros l; destruct l; auto.
-intros l; destruct l; auto.
 intros l1 l2 l3; destruct l1, l2, l3; auto.
 intros l1 l2; destruct l1, l2; auto.
-intuition.
-intuition.
+by [].
+by [].
 intros l1 l2; destruct l1, l2; auto.
 intros l1 l2; destruct l1, l2; auto.
 intros l1 l2 l; destruct l1, l2, l; auto.
@@ -37,5 +42,5 @@ Defined.
 Instance Lattice_Lab2 : Lattice Lab2 := { top := H }.
 Proof. intros l; destruct l; auto. Defined.
 
-Instance FiniteLattice_Lab2 : FiniteLattice Lab2 := { elems := [L;H] }.
-Proof. intros l; destruct l; simpl; tauto. Defined.
+Instance FiniteLattice_Lab2 : FiniteLattice Lab2 := { elems := [:: L;H] }.
+Proof. by case. Defined.
