TestingCommon.v
@@ -1,4 +1,3 @@
-Require Import List. Import ListNotations.
 Require Import ZArith.
 Require Import String.
 Require Import NPeano.
